src/tls/NewHandshake.fsti
@@ -1,0 +1,519 @@
+module NewHandshake
+
+(*** Updated Interface (Temp File) ***)
+
+// current limitations: 
+// - no abstract type for encrypted handshake traffic
+// - no support for 0RTT and false-start
+// - partnering between handshakes is static (needs fixing)
+
+open FStar.Heap
+open FStar.HyperHeap
+//FIXME! Don't open so much ... gets confusing. Use module abbrevs instead
+open FStar.Seq
+open FStar.SeqProperties // for e.g. found
+open FStar.Set  
+
+open Platform.Error
+open Platform.Bytes
+
+open TLSError
+open TLSInfo
+open TLSConstants
+open Range
+open HandshakeMessages
+open HSCrypto
+open StAE
+
+module HH = HyperHeap
+module MS = MonotoneSeq
+module MR = FStar.Monotonic.RRef
+
+// represents the outcome of a successful handshake, 
+// providing context for the derived epoch
+type handshake = 
+  | Fresh of sessionInfo
+  | Resumed of abbrInfo * sessionInfo //changed: was hs * seq epoch (creating cycle)
+// We use SessionInfo as unique session indexes.
+// We tried using instead hs, but this creates circularities
+// We'll probably need a global log to reason about them.
+// We should probably do the same in the session store.
+
+
+// extracts a transport key identifier from a handshake record
+val hsId: handshake -> Tot (i:id { is_stream_ae i }) //16-05-19 focus on TLS 1.3
+
+//<expose for TestClient>
+val ri : Type0
+type b_log = bytes 
+//or how about: 
+//type log = list (m:bytes{exists ht d. m = messageBytes ht d})
+type eph_s = option kex_s_priv
+type eph_c = list kex_s_priv
+type nego = {
+     n_resume: bool;
+     n_client_random: TLSInfo.random;
+     n_server_random: TLSInfo.random;
+     n_sessionID: option sessionID;
+     n_protocol_version: protocolVersion;
+     n_kexAlg: TLSConstants.kexAlg;
+     n_aeAlg: TLSConstants.aeAlg;
+     n_sigAlg: option TLSConstants.sigAlg;
+     n_cipher_suite: cipherSuite;
+     n_dh_group: option namedGroup;
+     n_compression: option compression;
+     n_extensions: negotiatedExtensions;
+     n_scsv: list scsv_suite;
+}                 
+
+type hs_id = {
+     id_cert: Cert.chain;
+     id_sigalg: option sigHashAlg;
+}
+
+type ake = {
+     ake_server_id: option hs_id;
+     ake_client_id: option hs_id;
+     ake_pms: bytes;
+     ake_session_hash: bytes;
+     ake_ms: bytes;
+}
+
+type session = {
+     session_nego: nego;
+     session_ake: ake;
+}     
+
+val prepareClientHello: config -> KeySchedule.ks -> HandshakeLog.log -> option ri -> option sessionID -> ST (hs_msg * bytes)
+  (requires (fun h -> True))
+  (ensures (fun h0 i h1 -> True))
+val prepareServerHello: config -> KeySchedule.ks -> HandshakeLog.log -> option ri -> (hs_msg * bytes) -> ST (result (nego * (hs_msg * bytes)))
+  (requires (fun h -> True))
+  (ensures (fun h0 i h1 -> True))
+val processServerHello: c:config -> KeySchedule.ks -> HandshakeLog.log -> option ri -> ch -> (hs_msg * bytes) ->
+                        ST (result (nego * option KeySchedule.recordInstance))
+  (requires (fun h -> True))
+  (ensures (fun h0 i h1 -> True))
+
+
+//</expose for TestClient>
+
+// relocate?
+type fresh_subregion r0 r h0 h1 = fresh_region r h0 h1 /\ extends r r0
+
+type epoch_region_inv (#i:id) (hs_rgn:rgn) (r:reader (peerId i)) (w:writer i) =
+  disjoint hs_rgn (region w)                  /\
+  parent (region w) <> FStar.HyperHeap.root    /\
+  parent (region r) <> FStar.HyperHeap.root    /\
+  parent hs_rgn = parent (parent (region w))  /\ //Grandparent of each writer is a sibling of the handshake
+  disjoint (region w) (region r)              /\
+  is_epoch_rgn (region w)                     /\ //they're all colored as epoch regions
+  is_epoch_rgn (region r)                     /\
+  is_epoch_rgn (parent (region w))            /\
+  is_epoch_rgn (parent (region r))            /\
+  is_hs_rgn hs_rgn                              //except for the hs_rgn, of course
+
+abstract type epoch_region_inv' (#i:id) (hs_rgn:rgn) (r:reader (peerId i)) (w:writer i) =
+  epoch_region_inv hs_rgn r w
+  
+module I = IdNonce
+
+type epoch (hs_rgn:rgn) (n:TLSInfo.random) = 
+  | Epoch: h: handshake ->
+           r: reader (peerId (hsId h)) ->
+           w: writer (hsId h) {epoch_region_inv' hs_rgn r w /\ I.nonce_of_id (hsId h) = n} 
+	   -> epoch hs_rgn n
+  // we would extend/adapt it for TLS 1.3,
+  // e.g. to notify 0RTT/forwad-privacy transitions
+  // for now epoch completion is a total function on handshake --- should be stateful
+
+let reveal_epoch_region_inv_all (u:unit)
+  : Lemma (forall i hs_rgn r w.{:pattern (epoch_region_inv' #i hs_rgn r w)}
+	   epoch_region_inv' #i hs_rgn r w
+	   <==>
+   	   epoch_region_inv #i hs_rgn r w)
+  = ()	   
+
+let reveal_epoch_region_inv (#hs_rgn:rgn) (#n:TLSInfo.random) (e:epoch hs_rgn n) 
+  : Lemma (let r = Epoch.r e in 
+	   let w = Epoch.w e in 
+	   epoch_region_inv hs_rgn r w)
+  = ()
+
+let writer_epoch (#hs_rgn:rgn) (#n:TLSInfo.random) (e:epoch hs_rgn n) 
+  : Tot (w:writer (hsId (e.h)) {epoch_region_inv hs_rgn (Epoch.r e) w})
+  = Epoch.w e
+
+let reader_epoch (#hs_rgn:rgn) (#n:TLSInfo.random) (e:epoch hs_rgn n) 
+  : Tot (r:reader (peerId (hsId (e.h))) {epoch_region_inv hs_rgn r (Epoch.w e)})
+  = match e with | Epoch h r w -> r //16-05-20 Epoch.r e failed.
+
+(* The footprint just includes the writer regions *)
+abstract let epochs_inv (#r:rgn) (#n:TLSInfo.random) (es: seq (epoch r n)) =
+  forall (i:nat { i < Seq.length es })
+    (j:nat { j < Seq.length es /\ i <> j}).{:pattern (Seq.index es i); (Seq.index es j)}
+    let ei = Seq.index es i in
+    let ej = Seq.index es j in
+    parent (region ei.w) = parent (region ej.w) /\  //they all descend from a common epochs sub-region of the connection
+    disjoint (region ei.w) (region ej.w)           //each epoch writer lives in a region disjoint from the others
+ 
+let epochs (r:rgn) (n:TLSInfo.random) = es: seq (epoch r n) { epochs_inv es }
+
+
+// internal stuff: state machine, reader/writer counters, etc.
+// (will take other HS fields as parameters)
+val handshake_state : role -> Type0
+(* #reset-options "--z3timeout 3 --initial_fuel 2 --max_fuel 2 --initial_ifuel 2 --max_ifuel 2" *)
+
+let resume_id (r:role) = o:option sessionID{r=Server ==> o=None}
+
+type hs =
+  | HS: #region: rgn { is_hs_rgn region } ->
+              r: role ->
+         resume: resume_id r ->
+            cfg: config ->
+          nonce: TLSInfo.random ->  // unique for all honest instances; locally enforced; proof from global HS invariant? 
+            log: MS.i_seq region (epoch region nonce) epochs_inv ->  // append-only, monotonic log of epochs
+          state: rref region (handshake_state r)  ->       // opaque, subject to invariant
+             hs
+
+
+(* the handshake internally maintains epoch 
+   indexes for the current reader and writer *)
+
+let logT (s:hs) (h:HyperHeap.t) = MS.i_sel h s.log
+
+let stateType (s:hs) = epochs s.region s.nonce * handshake_state (HS.r s)
+
+let stateT (s:hs) (h:HyperHeap.t) : stateType s = (logT s h, sel h s.state)
+
+let non_empty h s = Seq.length (logT s h) > 0
+
+let logIndex (#t:Type) (log: seq t) = n:int { -1 <= n /\ n < Seq.length log }
+
+// returns the current index in the log for reading or writing, or -1 if there is none.
+// depends only on the internal state of the handshake
+val iT0: s:hs -> rw:rw -> st:stateType s -> Tot (logIndex (fst st))
+let iT s rw h = iT0 s rw (stateT s h) 
+
+//A framing lemma with a very trivial proof, because of the way stateT abstracts the state-dependent parts
+let frame_iT_trivial  (s:hs) (rw:rw) (h0:HH.t) (h1:HH.t) 
+  : Lemma (stateT s h0 = stateT s h1
+           ==> iT s rw h0 = iT s rw h1) 
+  = ()	                               
+
+//Here's a framing on stateT connecting it to the region discipline
+let frame_stateT  (s:hs) (rw:rw) (h0:HH.t) (h1:HH.t) (mods:Set.set rid)
+  : Lemma (requires HH.modifies_just mods h0 h1
+		    /\ Map.contains h0 s.region
+		    /\ not (Set.mem s.region mods))
+          (ensures stateT s h0 = stateT s h1)
+  = ()	                               
+
+//This is probably the framing lemma that a client of this module will want to use
+let frame_iT  (s:hs) (rw:rw) (h0:HH.t) (h1:HH.t) (mods:Set.set rid)
+  : Lemma (requires HH.modifies_just mods h0 h1
+		    /\ Map.contains h0 s.region
+		    /\ not (Set.mem s.region mods))
+          (ensures stateT s h0 = stateT s h1
+		   /\ iT s rw h0 = iT s rw h1)
+  = frame_stateT s rw h0 h1 mods;
+    frame_iT_trivial s rw h0 h1
+    
+// returns the epoch for reading or writing
+let eT s rw (h:HyperHeap.t { iT s rw h >= 0 }) = Seq.index (logT s h) (iT s rw h)
+
+let readerT s h = eT s Reader h 
+let writerT s h = eT s Writer h
+
+// this function increases (how to specify it once for all?)
+val i: s:hs -> rw:rw -> ST int 
+  (requires (fun h -> True))
+  (ensures (fun h0 i h1 -> h0 = h1 /\ i = iT s rw h1))
+
+val processServerHelloDone: cfg:config -> nego:nego -> ks:KeySchedule.ks -> log:HandshakeLog.log ->
+    			    list (hs_msg*bytes) -> list (hs_msg * bytes) -> ST (result (list (hs_msg * bytes)))
+  (requires (fun h -> nego.n_protocol_version <> TLS_1p3))
+  (ensures (fun h0 i h1 -> True))
+val prepareClientFinished: KeySchedule.ks -> HandshakeLog.log -> ST (hs_msg * bytes)
+  (requires (fun h -> True))
+  (ensures (fun h0 i h1 -> True))
+val processServerFinished: KeySchedule.ks -> HandshakeLog.log -> (hs_msg * bytes) -> ST (result bytes)
+  (requires (fun h -> True))
+  (ensures (fun h0 i h1 -> True))
+
+val processServerFinished_13: cfg:config -> n:nego -> ks:KeySchedule.ks -> log:HandshakeLog.log ->
+    			      list (hs_msg*bytes) -> ST (result (list (hs_msg * bytes) * bytes * KeySchedule.recordInstance))
+  (requires (fun h -> True))
+  (ensures (fun h0 i h1 -> True))
+
+
+// name-clashing
+// let reader s = i s Reader
+// let writer s = i s Reader
+
+
+let forall_epochs (hs:hs) h (p:(epoch hs.region hs.nonce -> Type)) = 
+  (let es = logT hs h in
+   forall (i:nat{i < Seq.length es}).{:pattern (Seq.index es i)} p (Seq.index es i))
+     
+(* //vs modifies clauses? *)
+(* let unmodified_epochs s h0 h1 =  *)
+(*   forall_epochs s h0 (fun e ->  *)
+(*     let rs = regions e in  *)
+(*     (forall (r:rid{Set.mem r rs}).{:pattern (Set.mem r rs)} Map.sel h0 r = Map.sel h1 r)) *)
+
+//epochs in h1 extends epochs in h0 by one 
+let fresh_epoch h0 s h1 =
+  let es0 = logT s h0 in 
+  let es1 = logT s h1 in 
+  Seq.length es1 > 0 &&
+  es0 = Seq.slice es1 0 (Seq.length es1 - 1)
+
+let latest h (s:hs{Seq.length (logT s h) > 0}) = // accessing the latest epoch
+ let es = logT s h in
+ Seq.index es (Seq.length es - 1)
+
+// separation policy: the handshake mutates its private state, 
+// only depends on it, and only extends the log with fresh epochs.
+
+
+// placeholder, to be implemented as a stateful property.
+assume val completed: #region:rgn -> #nonce:TLSInfo.random -> epoch region nonce -> Type0
+
+// consider adding an optional (resume: option sid) on the client side
+// for now this bit is not explicitly authenticated.
+
+// Well-formed logs are all prefixes of (Epoch; Complete)*; Error
+// This crucially assumes that TLS keeps track of OutCCS and InCCSAck
+// so that it knows which reader & writer to use (not always the latest ones):
+// - within InCCSAck..OutCCS, we still use the older writer
+// - within OutCCS..InCCSAck, we still use the older reader
+// - otherwise we use the latest readers and writers
+
+// technicality: module dependencies?
+// we used to pre-declare all identifiers in TLSInfo
+// we used owe could also record (fatal) errors as log terminators
+ 
+// abstract invariant; depending only on the HS state (not the epochs state)
+// no need for an epoch states invariant here: the HS never modifies them
+ 
+assume val hs_invT : s:hs -> epochs:seq (epoch s.region s.nonce) -> handshake_state (HS.r s) -> Type0
+
+let hs_inv (s:hs) (h: HyperHeap.t) = 
+  hs_invT s (logT s h) (sel h (HS.state s))  //An abstract invariant of HS-internal state
+  /\ MS.i_contains s.log h                    //Nothing deep about these next two, since they can always 
+  /\ HyperHeap.contains_ref s.state h                 //be recovered by 'recall'; carrying them in the invariant saves the trouble
+
+//TODO: need a lemma to frame hs_inv across updates that don't clash with HS.region
+//TODO: need a lemma to frame a write to one epoch across the state of the other epochs
+
+// returns the protocol version negotiated so far
+// (used for formatting outgoing packets, but not trusted)
+val version: s:hs -> ST protocolVersion
+  (requires (hs_inv s))
+  (ensures (fun h0 pv h1 -> h0 = h1))
+
+
+(* used to be part of TLS.pickSendPV, with 3 cases: 
+
+   (1) getMinVersion hs; then 
+   (2) fixed by ServerHello; then
+   (3) read from the current writing epoch
+
+   val epoch_pv: #region:rid -> #peer:rid -> epoch region peer -> Tot ProtocolVersion
+
+   Instead, we could add an invariant: for all epochs e in hs.log, we have epoch_pv e = version hs.
+*)
+
+
+(*** Control Interface ***)
+
+// Create instance for a fresh connection, with optional resumption for clients
+val init: r0:rid -> r: role -> cfg:config -> resume: resume_id r -> 
+  ST hs
+  (requires (fun h -> True))
+  (ensures (fun h0 s h1 ->
+    modifies Set.empty h0 h1 /\
+    fresh_subregion r0 (HS.region s) h0 h1 /\
+    hs_inv s h1 /\
+    HS.r s = r /\
+    HS.resume s = resume /\
+    HS.cfg s = cfg /\
+    logT s h1 = Seq.createEmpty ))
+
+let mods s h0 h1 = 
+  HyperHeap.modifies_one s.region h0 h1
+  
+let modifies_internal h0 s h1 =
+    hs_inv s h1 /\
+    mods s h0 h1 /\ 
+    modifies_rref s.region !{as_ref s.state} h0 h1
+
+// Idle client starts a full handshake on the current connection
+val rehandshake: s:hs -> config -> ST bool
+  (requires (fun h -> hs_inv s h /\ HS.r s = Client))
+  (ensures (fun h0 _ h1 -> modifies_internal h0 s h1))
+
+// Idle client starts an abbreviated handshake resuming the current session
+val rekey: s:hs -> config -> ST bool
+  (requires (fun h -> hs_inv s h /\ HS.r s = Client))
+  (ensures (fun h0 _ h1 -> modifies_internal h0 s h1))
+
+// (Idle) Server requests an handshake
+val request: s:hs -> config -> ST bool
+  (requires (fun h -> hs_inv s h /\ HS.r s = Server))
+  (ensures (fun h0 _ h1 -> modifies_internal h0 s h1))
+
+val invalidateSession: s:hs -> ST unit
+  (requires (hs_inv s))
+  (ensures (fun h0 _ h1 -> modifies_internal h0 s h1)) // underspecified
+
+
+(*** Outgoing ***)
+
+// payload of a handshake fragment, to be made opaque eventually
+type message (i:id) = (| rg: frange i & rbytes rg |)
+
+// What the HS asks the record layer to do, in that order.
+type outgoing (i:id) (* initial index *) = 
+  | Outgoing: 
+      send_first: option (message i) -> // HS fragment to be sent;  (with current id)
+      send_ccs  : bool               -> // CCS fragment to be sent; (with current id)
+      next_keys : bool               -> // the writer index increases;
+      complete  : bool               -> // the handshake is complete!
+      outgoing i 
+  | OutError: error -> outgoing i       // usage? in case something goes wrong when preparing messages. 
+
+let out_next_keys (#i:id) (r:outgoing i) = is_Outgoing r && Outgoing.next_keys r
+let out_complete (#i:id) (r:outgoing i)  = is_Outgoing r && Outgoing.complete r
+
+let next_fragment_ensures (#i:id) (s:hs) h0 (result:outgoing i) h1 = 
+    let es = logT s h0 in
+    let w0 = iT s Writer h0 in
+    let w1 = iT s Writer h1 in
+    let r0 = iT s Reader h0 in
+    let r1 = iT s Reader h1 in
+    hs_inv s h1 /\
+    mods s h0 h1 /\
+    r1 == r0 /\
+//  w1 == (match result with | Outgoing _ _ true _ -> w0 + 1 | _ -> w0 ) /\
+    w1 == (if out_next_keys result then  w0 + 1 else w0 ) /\
+    (b2t (out_complete result) ==> w1 >= 0 /\ r1 = w1 /\ iT s Writer h1 >= 0 /\ completed (eT s Writer h1)) 
+
+val next_fragment: i:id -> s:hs -> ST (outgoing i)
+  (requires (fun h0 -> 
+    let es = logT s h0 in
+    let j = iT s Writer h0 in 
+    hs_inv s h0 /\
+    (if j = -1 then i = noId else let e = Seq.index es j in i = hsId e.h)   
+  ))
+  (ensures (next_fragment_ensures s))
+
+//<expose for TestClient>
+val parseHandshakeMessages : option protocolVersion -> option kexAlg -> buf:bytes -> Tot  (result (rem:bytes * list (hs_msg * bytes)))
+//</expose for TestClient>
+
+
+(*** Incoming ***)
+
+type incoming = 
+  // the fragment is accepted, and...
+  | InAck: 
+      next_keys : bool -> // the reader index increases;
+      complete  : bool -> // the handshake is complete!
+      incoming
+
+  | InQuery: Cert.chain -> bool -> incoming // could be part of InAck if no explicit user auth
+  | InError: error -> incoming // how underspecified should it be?
+
+let in_next_keys (r:incoming) = is_InAck r && InAck.next_keys r
+let in_complete (r:incoming)  = is_InAck r && InAck.complete r
+
+let recv_ensures (s:hs) (h0:HyperHeap.t) (result:incoming) (h1:HyperHeap.t) = 
+    let w0 = iT s Writer h0 in
+    let w1 = iT s Writer h1 in
+    let r0 = iT s Reader h0 in
+    let r1 = iT s Reader h1 in
+    hs_inv s h1 /\
+    mods s h0 h1 /\
+    w1 == w0 /\
+    r1 == (if in_next_keys result then r0 + 1 else r0) /\
+    (b2t (in_complete result) ==> r1 >= 0 /\ r1 = w1 /\ iT s Reader h1 >= 0 /\ completed (eT s Reader h1))
+
+val recv_fragment: s:hs -> #i:id -> message i -> ST incoming
+  (requires (hs_inv s))
+  (ensures (recv_ensures s))
+
+val recv_ccs: s:hs -> ST incoming  // special case: CCS before 1p3; could merge with recv_fragment
+  (requires (hs_inv s)) // could require pv <= 1p2
+  (ensures (fun h0 result h1 ->
+    ~(is_InQuery result) /\ recv_ensures s h0 result h1 ))
+
+val authorize: s:hs -> Cert.chain -> ST incoming // special case: explicit authorize (needed?)
+  (requires (hs_inv s))
+  (ensures (fun h0 result h1 ->
+    (is_InAck result \/ is_InError result) /\ recv_ensures s h0 result h1 ))
+    
+
+(* working notes towards covering both TLS 1.2 and 1.3, with 0RTT and falsestart
+
+type sendMsg (i:id) = // writer-indexed
+  | OutHS:
+       rg:frange_any ->
+       fragment i rg rbytes rg -> // first write this Handshake fragment, then
+       next:bool     ->           // signal increment of the writer index
+       finished:bool ->           // enable false-start sending (after sending this 1st Finished)
+       complete:bool ->           // signal completion (after sending this 2nd Finished)
+       outbox
+  | OutCCS  // before TLS 1.3; same semantics as above with explicit CCS (true, false, false)
+  | OutIdle // nothing to do
+
+(* e.g. in TLS 1.3 1RTT server sends OutHS (Finished ...) next
+                   0RTT server sends OutHS (Finished ...) next finished  (if 0.5RTT is enabled)
+                   then client sends OutHS (Finished ...) next complete
+
+        in TLS 1.2 full server sends OutHS (Finished ...) finished
+                   then client sends OutHS (Finished ...) complete
+                   sending CCS implicitly says next  *)
+
+type recvMsg =
+  | InAck:
+       next:bool ->      // signal increment of the reader index (before receiving the next packet)
+       finished:bool ->  // enable false-start receiving (in TLS 1.2, as we accepted the 1st Finished)
+       complete:bool ->  // signal completion (as we accepted the 2nd Finished)
+       inbox
+  | InQuery of Cert.chain * bool  // asks for authorization (all flags cleared; will have cases)
+  | InError of error
+
+(* e.g. in TLS 1.3 1RTT client accepts Finished: InAck next
+                   0RTT client accepts Finished: InAck next finished  (if 0.5RTT is enabled)
+                   then server accepts Finished: InAck next complete
+
+        in TLS 1.2 full server accepts Finished: InAck finished
+                   then client accepts Finished: InAck complete
+                   accepting CCS returns:        InAck next  *)
+
+Not sure how to handle 0RTT switches.
+"end_of_early_data" is not HS.
+On the receiving server side,
+- After processing ClientHello, HS signals switch to 0RTT-HS (or jump to 1RTT_HS) receive keys.
+- After processing Finished0, HS signals switch to 0RTT-AD
+- After receiving EED, the record calls HS, which signals switch to 1RTT-HS [too early?]
+- After receiving Finished, HS signals switch to 1RTT-AD.
+
+[a proper use of index 0]
+
+If we introduce dummy reverse streams (specified to remain empty), we still have to interpret
+the first client receive++ as +=3.
+What would trigger it? a locally-explicit CCS after accepting the ServerHello.
+
+
+Otherwise the "next" mechanism seems fine; we just bump a ghost index
+from 2 to 4 by the time we reach AD.
+
+Also 1.3 trouble for sending HS-encrypted data immediately *after* next:
+we can increment after sending ClientHello, but we don't have the epoch yet!
+
+Ad hoc cases? or just an extra case?
+In fact, ~ keeping a local, explicit CCS signal. *)
